trying to fix the typechecking stuff

theories/examples/set.v
@@ -38,7 +38,7 @@ Definition lookup_loop : expr :=
   rec: "lookup_loop" "arr" "k" "l" "r" "x" "is_found" :=
   if: "k" = #0 then "is_found"
   else let: "i" := BinOp QuotOp ("l" + "r") #2 in
-       let: "elem" := "get" "arr" "i" NONE in
+       let: "elem" := "get" "arr" "i" in
        let: "lr1" := ("i"+#1, "r") in
        let: "lr2" := ("l", "i"-#1) in
        let: "lr" := if: (lte_option "elem" "x")
@@ -96,17 +96,28 @@ Qed.
 
 
 Lemma If_typed_flat' 𝔏 ξ Γ e1 e2 e3 τ :
+  ξ ≠ High →
   almost_val (dom stringset Γ) e2 →
   almost_val (dom stringset Γ) e3 →
-  ξ ≠ High →
-  has_type 𝔏 ξ Γ e1 (tbool High) →
   has_type 𝔏 ξ Γ e2 τ →
-  has_type 𝔏 ξ Γ e3 τ →
   flat_type τ →
+  has_type 𝔏 ξ Γ e3 τ →
+  has_type 𝔏 ξ Γ e1 (tbool High) →
   has_type 𝔏 ξ Γ (if: e1 then e2 else e3) τ.
 Proof.
   intros. by apply If_typed_flat.
 Qed.
+
+Lemma If_typed' 𝔏 ξ Γ e1 e2 e3 τ :
+  has_type 𝔏 ξ Γ e1 (tbool Low) →
+  has_type 𝔏 ξ Γ e2 τ →
+  has_type 𝔏 ξ Γ e3 τ →
+  has_type 𝔏 ξ Γ (if: e1 then e2 else e3) τ.
+Proof.
+  intros. eapply If_typed; try done. by destruct ξ.
+Qed.
+
+
 
 Existing Instance singleton_binder.
 Existing Instance insert_binder.
@@ -124,8 +135,8 @@ Proof.
 Qed.
 
 Lemma App_typed' 𝔏 ξ Γ e1 e2 τ τ' :
-  has_type 𝔏 ξ Γ e1 (τ → τ')%ty →
   has_type 𝔏 ξ Γ e2 τ →
+  has_type 𝔏 ξ Γ e1 (τ → τ')%ty →
   has_type 𝔏 ξ Γ (App e1 e2) τ'.
 Proof.
   intros. rewrite -(stamp_low τ').
@@ -155,9 +166,22 @@ Hint Constructors bin_op_bool : typed.
 Hint Constructors bin_op_int_bool : typed.
 Hint Constructors flat_type : typed.
 Hint Constructors almost_val : typed.
-Hint Extern 10 (<[_:=_]>_ !! _ = Some _) => eapply lookup_insert : typed.
-Hint Extern 20 (<[_:=_]>_ !! _ = Some _) => rewrite lookup_insert_ne; last done : typed.
-Hint Extern 10 (_ ∈ _) => rewrite ?insert_empty_binder ?insert_string_binder; set_solver : typed.
+
+Hint Extern 10 (<[_:=_]>_ !! _ = Some _) =>
+  rewrite ?insert_empty_binder ?insert_string_binder ;
+  eapply lookup_insert : typed.
+Hint Extern 20 (<[_:=_]>_ !! _ = Some _) =>
+  rewrite ?insert_empty_binder ?insert_string_binder ;
+  rewrite lookup_insert_ne; last done : typed.
+
+Hint Extern 20 (_ ∈ _) =>
+  rewrite ?insert_empty_binder ?insert_string_binder ;
+  (apply elem_of_union_l || apply elem_of_union_r) ;
+  set_solver : typed.
+
+Hint Extern 1 (_ ∈ dom _ _) =>
+  (* rewrite ?insert_empty_binder ?insert_string_binder; *)
+  apply elem_of_dom ; simplify_map_eq ; eexists ; done : typed.
 
 Hint Extern 10 (_ ⊔ _ ⊑ _) => rewrite (left_id Low); reflexivity.
 Hint Extern 10 (_ ⊔ _ ⊑ _) => rewrite (right_id Low); reflexivity.
@@ -170,6 +194,8 @@ Remove Hints BinOp_bool_typed : typed.
 Hint Resolve BinOp_bool_typed' : typed.
 Remove Hints BinOp_int_bool_typed : typed.
 Hint Resolve BinOp_int_bool_typed' : typed.
+Remove Hints If_typed : typed.
+Hint Resolve If_typed' | 20 : typed.
 Remove Hints If_typed_flat : typed.
 Hint Resolve If_typed_flat' : typed.
 Remove Hints Match_typed_flat : typed.
@@ -184,7 +210,10 @@ Section typed.
   Variable 𝔏 : gset loc.
   Variable arr_t : type.
   Definition ctx : stringmap type :=
-    <["get":=(arr_t → tint High → tintoption High High → tintoption High High)%ty]>{["make":=(tunit → arr_t)%ty]}.
+    <["get":=(arr_t → tint High → tintoption High High)%ty]>{["make":=(tunit → arr_t)%ty]}.
+
+  Definition ctx_ Γ : stringmap type :=
+    <["get":=(arr_t → tint High → tintoption High High)%ty]>(<["make":=(tunit → arr_t)%ty]>Γ).
 
   Lemma cap_typed Γ : has_type 𝔏 Low Γ cap (tint Low → tint Low).
   Proof.
@@ -196,17 +225,7 @@ Section typed.
                                     tint High →
                                     tbool High).
   Proof.
-    unfold eq_option.
-    eapply Rec_typed'; eauto with typed.
-    eapply Rec_typed'; eauto with typed.
-    eapply App_typed'; eauto with typed.
-    eapply Rec_typed'; eauto with typed.
-    eapply App_typed'; eauto 20 with typed.
-    (* XXX *)
-    eapply Match_typed_flat'; eauto with typed.
-    constructor. rewrite ?insert_empty_binder ?insert_string_binder.
-    rewrite (dom_insert_L _ "v1" (D:=stringset)).
-    set_solver.
+    unfold eq_option. eauto 30 with typed.
   Qed.
 
   Lemma lte_option_typed Γ : has_type 𝔏 Low Γ lte_option
@@ -214,36 +233,24 @@ Section typed.
                                     tint High →
                                     tbool High).
   Proof.
-    unfold lte_option. eauto 50 with typed.
+    unfold lte_option. eauto 30 with typed.
   Qed.
 
   Hint Resolve cap_typed : typed.
   Hint Resolve eq_option_typed : typed.
   Hint Resolve lte_option_typed : typed.
 
-  Lemma lookup_loop_typed : has_type 𝔏 Low ctx lookup_loop
-    (arr_t → tint Low → tint High → tint High → tint High → tbool High → tbool High).
+  Lemma lookup_loop_typed Γ :
+    Γ !! "get" = Some (arr_t → tint High → tintoption High High)%ty →
+    has_type 𝔏 Low Γ lookup_loop
+             (arr_t → tint Low → tint High → tint High → tint High → tbool High → tbool High).
   Proof.
-    unfold lookup_loop.
-    repeat eapply Rec_typed'; eauto with typed.
-    eapply If_typed; eauto with typed.
-    eapply App_typed'; eauto with typed.
-    eapply Rec_typed'; eauto with typed.
-    eapply App_typed'; eauto 20 with typed.
-    eapply Rec_typed'; eauto with typed.
-    eapply App_typed'; eauto with typed.
-    eapply Rec_typed'; eauto with typed.
-    eapply App_typed'; eauto with typed.
-    eapply Rec_typed'; eauto with typed.
-    eapply App_typed'; eauto with typed.
-    2:{ eapply If_typed_flat'; eauto with typed. }
-    eauto 100 with typed.
-    (* eapply Rec_typed'; eauto with typed. *)
-    (* eapply App_typed'; eauto with typed. *)
-    (* eapply Rec_typed'; eauto with typed. *)
-    (* eapply App_typed'; eauto with typed. *)
-    (* eapply Rec_typed'; eauto with typed. *)
-    (* eapply App_typed'; eauto 20 with typed. *)
+    intros. unfold lookup_loop.
+    repeat eapply Rec_typed'.
+    eapply If_typed';[eauto 10 with typed..|].
+    eapply App_typed'; first eauto 10 with typed.
+    eapply Rec_typed'.
+    eapply App_typed'; eauto 500 with typed.
   Qed.
 
 
